Bank.v
@@ -6,6 +6,8 @@ Require Import
   Coq.FSets.FMapList
   Coq.Structures.OrderedTypeEx.
 
+Require String.
+
 Module Import NatDict := FMapList.Make(Nat_as_OT).
 
 Section Bank.
@@ -37,16 +39,13 @@ Section Bank.
   Inductive Msg :=
   | req  : ReqMsg  -> Msg
   | resp : RespMsg -> Msg.
-  Definition Msg_eq_dec : forall m m' : Msg, {m = m'} + {m <> m'}.
-    repeat decide equality.
-  Defined.
 
   Inductive Input :=
   | Timeout
-  | Create    : Account -> Input
-  | Deposit   : Account -> Value -> Input
-  | Withdraw  : Account -> Value -> Input
-  | Check     : Account -> Input.
+  | Create   : Account -> Input
+  | Deposit  : Account -> Value -> Input
+  | Withdraw : Account -> Value -> Input
+  | Check    : Account -> Input.
 
   Inductive Output :=
   | Failed
@@ -59,77 +58,90 @@ Section Bank.
   Definition InitState (name : Name) : State :=
     mkState pass (NatDict.empty Value).
 
-  Definition StateHandler := GenHandler (Name * Msg) State Output unit.
+  Definition NetId     := String.string.
+  Inductive  NetMsg    := netM : NetId -> Msg    -> NetMsg.
+  Inductive  NetInput  := netI : NetId -> Input  -> NetInput.
+  Inductive  NetOutput := netO : NetId -> Output -> NetOutput.
+  Definition NetMsg_eq_dec : forall m m' : NetMsg, {m = m'} + {m <> m'}.
+    repeat decide equality.
+  Defined.
 
-  Definition ClientNetHandler (m : Msg) : StateHandler :=
+  Definition StateHandler := GenHandler (Name * NetMsg) State NetOutput unit.
+
+  Definition ClientNetHandler (nm : NetMsg) : StateHandler :=
     state <- get ;;
     let s := server state in
+    let 'netM id m := nm in
     match m with
     | req  _ => nop
     | resp r => match r with
-                | FailMsg     => put (mkState fail s)
-                | PassMsg _ _ => put (mkState pass s)
+                | FailMsg         => put (mkState fail s)
+                                     >> write_output (netO id Failed)
+                | PassMsg acc val => put (mkState pass s)
+                                     >> write_output (netO id (Passed acc val))
                 end
     end.
 
-  Definition ClientIOHandler (i : Input) : StateHandler :=
+  Definition ClientIOHandler (ni : NetInput) : StateHandler :=
     state <- get ;;
+    let 'netI id i := ni in
     let s := server state in (
       put (mkState wait s) ;;
       match i with
       | Timeout          => put (mkState fail s)
-      | Create   acc     => send (Server, req (CreateMsg   acc))
-      | Deposit  acc val => send (Server, req (DepositMsg  acc val))
-      | Withdraw acc val => send (Server, req (WithdrawMsg acc val))
-      | Check    acc     => send (Server, req (CheckMsg    acc))
+      | Create   acc     => send (Server, netM id (req (CreateMsg   acc)))
+      | Deposit  acc val => send (Server, netM id (req (DepositMsg  acc val)))
+      | Withdraw acc val => send (Server, netM id (req (WithdrawMsg acc val)))
+      | Check    acc     => send (Server, netM id (req (CheckMsg    acc)))
       end).
 
-  Definition ServerNetHandler (m : Msg) : StateHandler :=
+  Definition ServerNetHandler (nm : NetMsg) : StateHandler :=
     state <- get ;;
     let c := client state in
     let s := server state in
+    let 'netM id m := nm in
     match m with
     | resp _ => nop
     | req  r =>
         match r with
-        | CreateMsg acc => 
+        | CreateMsg acc =>
             match NatDict.find acc s with
             | None => let val'' := 0 in (
                         put (mkState c (NatDict.add acc val'' s))
-                        >> send (Client, resp (PassMsg acc val'')))
-            | _    => send (Client, resp FailMsg)
+                        >> send (Client, netM id (resp (PassMsg acc val''))))
+            | _    => send (Client, netM id (resp FailMsg))
             end
-        | DepositMsg acc val => 
+        | DepositMsg acc val =>
             match NatDict.find acc s with
             | Some val' => let val'' := val + val' in (
                              put (mkState c (NatDict.add acc val'' s))
-                             >> send (Client, resp (PassMsg acc val'')))
-            | _            => send (Client, resp FailMsg)
+                             >> send (Client, netM id (resp (PassMsg acc val''))))
+            | _            => send (Client, netM id (resp FailMsg))
             end
-        | WithdrawMsg acc val => 
+        | WithdrawMsg acc val =>
             match NatDict.find acc s with
             | Some val' => if lt_dec val val'
-                           then send (Client, resp FailMsg)
+                           then send (Client, netM id (resp FailMsg))
                            else let val'' := val' - val in (
                                   put (mkState c (NatDict.add acc val'' s))
-                                  >> send (Client, resp (PassMsg acc val'')))
-            | None      => send (Client, resp FailMsg)
+                                  >> send (Client, netM id (resp (PassMsg acc val''))))
+            | None      => send (Client, netM id (resp FailMsg))
             end
-        | CheckMsg acc => 
+        | CheckMsg acc =>
             match NatDict.find acc s with
-            | Some val' => send (Client, resp (PassMsg acc val'))
-            | None      => send (Client, resp FailMsg)
+            | Some val' => send (Client, netM id (resp (PassMsg acc val')))
+            | None      => send (Client, netM id (resp FailMsg))
             end
         end
     end.
 
-  Definition ServerIOHandler (m : Input) : StateHandler := nop.
+  Definition ServerIOHandler (ni : NetInput) : StateHandler := nop.
 
   Instance bank_base_params : BaseParams :=
   {
     data   := State ;
-    input  := Input ;
-    output := Output
+    input  := NetInput ;
+    output := NetOutput
   }.
 
   Definition Nodes : list Name := [Server ; Client].
@@ -148,18 +160,18 @@ Section Bank.
     unfold Nodes, List.In. destruct n ; auto.
   Qed.
 
-  Definition NetHandler (dst src : Name) (m : Msg) (s : State) :=
+  Definition NetHandler (dst src : Name) (nm : NetMsg) (s : State) :=
     runGenHandler_ignore s (
       match dst with
-      | Client => ClientNetHandler m
-      | Server => ServerNetHandler m
+      | Client => ClientNetHandler nm
+      | Server => ServerNetHandler nm
       end).
 
-  Definition IOHandler (src : Name) (i : Input) (s : State) :=
+  Definition IOHandler (n : Name) (ni : NetInput) (s : State) :=
     runGenHandler_ignore s (
-      match src with
-      | Client => ClientIOHandler i
-      | Server => ServerIOHandler i
+      match n with
+      | Client => ClientIOHandler ni
+      | Server => ServerIOHandler ni
       end).
 
   Instance bank_multi_params : MultiParams bank_base_params :=
@@ -167,8 +179,8 @@ Section Bank.
     name := Name ;
     name_eq_dec := Name_eq_dec;
 
-    msg := Msg ;
-    msg_eq_dec := Msg_eq_dec;
+    msg := NetMsg ;
+    msg_eq_dec := NetMsg_eq_dec;
 
     nodes := Nodes ;
     no_dup_nodes := nodup_Nodes ;
@@ -177,5 +189,11 @@ Section Bank.
     init_handlers := InitState ;
     net_handlers := NetHandler ;
     input_handlers := IOHandler
+  }.
+
+  Definition reboot (state : State) : State := state.
+  Instance failure_params : FailureParams _ :=
+  {
+    reboot := reboot
   }.
 End Bank.
