README.md
@@ -1,18 +1,55 @@
 # Distributed Banking System
 
-A simple project to experiment with proving liveness properties in [Verdi][verdi].
+A simple project to experiment with proving liveness properties in
+[Verdi][verdi].
+
+It spawns a banking server which keeps the account records, and a trusted ATM
+to which clients can talk to, for making transactions.
+
+## Requirements
+
+Proofs:
+- `verdi`
+- `coq`
+
+Executable:
+- `ocamlbuild`
+- `ocamlfind`
+- `uuidm`
+- `verdi-runtime`
+
+(All of the above are `opam install`-able.)
 
 ## Extraction & Execution
 
 - `make` in the root directory to compile the proofs _and_ extract executable code
-- Running `Bank.native`:
+- Running the cluster using `Bank.native`:
 
 ```shell-script
-# Server listening for input on port 8100, talking to Client on 9100
+# Server listening for input on port 8100, talking to ATM on 9100
 $ ./Bank.native -me 0 -port 8100 -node 0,localhost:9100 -node 1,localhost:9101
 
-# Client listening for input on port 8101, talking to Server on 9101
+# ATM listening for input on port 8101, talking to Server on 9101
 $ ./Bank.native -me 1 -port 8101 -node 0,localhost:9100 -node 1,localhost:9101
 ```
+
+- User interactions: making transactions using the ATM can be made by connecting
+  to the port the ATM is listening on. For example:
+
+```shell-script
+# Connect to ATM
+$ socat tcp:localhost:8101 -
+CHECK 1001
+FAIL
+CREATE 1001
+PASS 1001 0
+DEPOSIT 1001 10
+PASS 1001 10
+CHECK 1001
+PASS 1001 10
+...
+```
+
+(or use `make bank.d.byte` for a debug-build)
 
 [verdi]: https://github.com/uwplse/verdi
